verso/src/verso-manual/VersoManual/Table.lean
@@ -194,15 +194,15 @@ meta def table : DirectiveExpanderOf TableConfig
     -- The table should be a list of lists. Extract them!
     let #[oneBlock] := contents
       | throwError "Expected a single unordered list"
-    let `(block|ul{$items*}) := oneBlock
+    let some outer := Lean.Doc.UnorderedListView.of oneBlock
       | throwErrorAt oneBlock "Expected a single unordered list"
-    let preRows ← items.mapM getLi
+    let preRows := outer.items.map (·.contents)
     let rows ← preRows.mapM fun blks => do
-      let #[oneInRow] := blks.filter (·.raw.isOfKind ``Lean.Doc.Syntax.ul)
+      let #[oneInRow] := blks.filter (·.raw.isOfKind ``Lean.Doc.Parser.Block.ul)
         | throwError "Each row should have exactly one list in it"
-      let `(block|ul{ $cellItems*}) := oneInRow
+      let some inner := Lean.Doc.UnorderedListView.of oneInRow
         | throwErrorAt oneInRow "Each row should have exactly one list in it"
-      cellItems.mapM getLi
+      pure (inner.items.map (·.contents))
     if h : rows.size = 0 then
       throwErrorAt oneBlock "Expected at least one row"
     else
@@ -217,7 +217,4 @@ meta def table : DirectiveExpanderOf TableConfig
       let blocks : Array (Syntax.TSepArray `term ",") ← flattened.mapM (·.mapM elabBlock)
       ``(Block.other (Block.table $(quote columns) $(quote cfg.header) $(quote cfg.name) $(quote cfg.alignment)) #[Block.ul #[$[Verso.Doc.ListItem.mk #[$blocks,*]],*]])
 
-where
-  getLi : Syntax → DocElabM (TSyntaxArray `block)
-    | `(list_item| * $content* ) => pure content
-    | other => throwErrorAt other "Expected list item"
+
