verso/src/verso/Verso/Doc/Elab/Inline.lean
@@ -21,7 +21,8 @@ set_option backward.privateInPublic false
 public def throwUnexpected [Monad m] [MonadError m] (stx : Syntax) : m α :=
   throwErrorAt stx "unexpected syntax{indentD stx}"
 
-public partial def elabInline (inline : TSyntax `inline) : DocElabM (TSyntax `term) :=
+public partial def elabInline (inline : TSyntax ``Lean.Doc.Parser.inline) :
+    DocElabM (TSyntax `term) :=
   withRef inline <| withFreshMacroScope <| withIncRecDepth <| do
   match inline.raw with
   | .missing =>
@@ -35,10 +36,12 @@ public partial def elabInline (inline : TSyntax `inline) : DocElabM (TSyntax `te
         withRef stxNew <|
           elabInline ⟨stxNew⟩
     | none =>
+      let some view := Lean.Doc.InlineView.of ⟨stx⟩
+        | throwUnexpected stx
       let exp ← inlineExpandersFor kind
       for e in exp do
         try
-          let termStx ← withFreshMacroScope <| e stx
+          let termStx ← withFreshMacroScope <| e view
           return termStx
         catch
           | ex@(.internal id) =>
