verso/src/verso/Verso/Doc/Helpers.lean
@@ -5,6 +5,7 @@ Author: David Thrane Christiansen
 -/
 module
 import Lean.DocString.Syntax
+public import Lean.DocString.View
 public import Lean.Exception
 public import Lean.Log
 
@@ -18,36 +19,39 @@ namespace Verso.Doc
 If {name}`inlines` contains exactly one code inline, its contents are returned. Throws an error
 otherwise.
 -/
-public def oneCodeStr [Monad m] [MonadError m] (inlines : Array (TSyntax `inline)) : m StrLit := do
+public def oneCodeStr [Monad m] [MonadError m]
+    (inlines : TSyntaxArray ``Lean.Doc.Parser.inline) : m Lean.Doc.VersoCode := do
   let #[code] := inlines
-    | (if inlines.size == 0 then (throwError ·) else (throwErrorAt (mkNullNode inlines) ·)) "Expected one code element"
-  let `(inline|code($code:str)) := code
+    | (if inlines.size == 0 then (throwError ·)
+       else (throwErrorAt (mkNullNode (inlines.map (·.raw))) ·)) "Expected one code element"
+  let some v := Lean.Doc.CodeView.of code
     | throwErrorAt code "Expected a code element"
-  return code
+  return v.content
 
 /--
 If {name}`inlines` contains exactly one code inline, its contents are returned. Otherwise, an error
 is logged and {name}`none` is returned.
 -/
 public def oneCodeStr? [Monad m] [MonadError m] [MonadLog m] [AddMessageContext m] [MonadOptions m]
-    (inlines : Array (TSyntax `inline)) : m (Option StrLit) := do
+    (inlines : TSyntaxArray ``Lean.Doc.Parser.inline) : m (Option Lean.Doc.VersoCode) := do
   let #[code] := inlines
     | if inlines.size == 0 then
         Lean.logError "Expected a code element"
       else
-        logErrorAt (mkNullNode inlines) "Expected one code element"
+        logErrorAt (mkNullNode (inlines.map (·.raw))) "Expected one code element"
       return none
-  let `(inline|code($code)) := code
+  let some v := Lean.Doc.CodeView.of code
     | logErrorAt code "Expected a code element"
       return none
-  return some code
+  return some v.content
 
 /--
 If {name}`inlines` contains exactly one Lean name, it is returned with its source location as an
 identifier. Otherwise, an error is thrown.
 -/
-public def oneCodeName [Monad m] [MonadError m] (inlines : Array (TSyntax `inline)) : m Ident := do
+public def oneCodeName [Monad m] [MonadError m]
+    (inlines : TSyntaxArray ``Lean.Doc.Parser.inline) : m Ident := do
   let code ← oneCodeStr inlines
-  let str := code.getString
+  let str := code.getVersoCode
   let name := if str.contains '.' then str.toName else Name.str .anonymous str
   return mkIdentFrom code name
